Saturation_Framework/Clausal_Inference_Systems.thy
@@ -1,0 +1,111 @@
+theory Clausal_Inference_Systems
+  imports
+    Standard_Redundancy_Criterion
+    Ordered_Resolution_Prover.Herbrand_Interpretation
+begin
+
+
+subsection \<open>Setup\<close>
+
+abbreviation true_lit_curvy :: "'a interp \<Rightarrow> 'a literal \<Rightarrow> bool" (infix "|\<approx>l" 50) where
+  "I |\<approx>l L \<equiv> I \<Turnstile>l L"
+
+abbreviation true_cls_curvy :: "'a interp \<Rightarrow> 'a clause \<Rightarrow> bool" (infix "|\<approx>" 50) where
+  "I |\<approx> C \<equiv> I \<Turnstile> C"
+
+abbreviation true_clss_curvy :: "'a interp \<Rightarrow> 'a clause set \<Rightarrow> bool" (infix "|\<approx>s" 50) where
+  "I |\<approx>s \<C> \<equiv> I \<Turnstile>s \<C>"
+
+abbreviation true_cls_mset_curvy :: "'a interp \<Rightarrow> 'a clause multiset \<Rightarrow> bool" (infix "|\<approx>m" 50) where
+  "I |\<approx>m \<C> \<equiv> I \<Turnstile>m \<C>"
+
+no_notation true_lit (infix "\<Turnstile>l" 50)
+no_notation true_cls (infix "\<Turnstile>" 50)
+no_notation true_clss (infix "\<Turnstile>s" 50)
+no_notation true_cls_mset (infix "\<Turnstile>m" 50)
+
+
+subsection \<open>Consequence Relation\<close>
+
+locale clausal_consequence_relation
+begin
+
+abbreviation Bot :: "'a clause set" where
+  "Bot \<equiv> {{#}}"
+
+definition entails :: "'a clause set \<Rightarrow> 'a clause set \<Rightarrow> bool" (infix "\<Turnstile>" 50) where
+  "N1 \<Turnstile> N2 \<longleftrightarrow> (\<forall>I. I |\<approx>s N1 \<longrightarrow> I |\<approx>s N2)"
+
+sublocale consequence_relation Bot entails
+proof
+  fix N2 N1 :: "'a clause set"
+  assume "N2 \<subseteq> N1"
+  then show "N1 \<Turnstile> N2"
+    unfolding entails_def using true_clss_mono by blast
+next
+  fix N2 N1 :: "'a clause set"
+  assume "\<forall>C \<in> N2. N1 \<Turnstile> {C}"
+  then show "N1 \<Turnstile> N2"
+    unfolding entails_def true_clss_singleton by (simp add: true_clss_def)
+qed (auto simp: entails_def)
+
+end
+
+locale clausal_cex_red_inference_system = inference_system Inf + clausal_consequence_relation
+  for Inf :: "('a :: wellorder) clause inference set" +
+  fixes clausal_I_of :: "'a clause set \<Rightarrow> 'a interp"
+  assumes clausal_Inf_cex_reducing:
+    "{#} \<notin> N \<Longrightarrow> D \<in> N \<Longrightarrow> \<not> clausal_I_of N |\<approx> D \<Longrightarrow>
+     (\<And>C. C \<in> N \<Longrightarrow> \<not> clausal_I_of N |\<approx> C \<Longrightarrow> D \<le> C) \<Longrightarrow>
+     \<exists>Cs E. set Cs \<subseteq> N \<and> clausal_I_of N |\<approx>s set Cs \<and> Infer (Cs @ [D]) E \<in> Inf
+        \<and> \<not> clausal_I_of N |\<approx> E \<and> E < D"
+begin
+
+definition clss_of_interp :: "'a set \<Rightarrow> 'a literal multiset set" where
+  "clss_of_interp I = {{#(if A \<in> I then Pos else Neg) A#} |A. True}"
+
+abbreviation I_of :: "'a clause set \<Rightarrow> 'a clause set" where
+  "I_of N \<equiv> clss_of_interp (clausal_I_of N)"
+
+lemma true_clss_of_interp_iff_equal[simp]: "J |\<approx>s clss_of_interp I \<longleftrightarrow> J = I"
+  unfolding clss_of_interp_def true_clss_def true_cls_def true_lit_def by force
+
+lemma entails_iff_models[simp]: "clss_of_interp I \<Turnstile> CC \<longleftrightarrow> I |\<approx>s CC"
+  unfolding entails_def by simp
+
+lemma Inf_cex_reducing:
+  assumes
+    bot_ni_n: "N \<inter> Bot = {}" and
+    d_in_n: "D \<in> N" and
+    n_ent_d: "\<not> I_of N \<Turnstile> {D}" and
+    d_min: "\<And>C. C \<in> N \<Longrightarrow> \<not> I_of N \<Turnstile> {C} \<Longrightarrow> D \<le> C"
+  shows "\<exists>\<iota> \<in> Inf.
+    main_prem_of \<iota> = D \<and> set (side_prems_of \<iota>) \<subseteq> N
+    \<and> I_of N \<Turnstile> set (side_prems_of \<iota>)
+    \<and> \<not> I_of N \<Turnstile> {concl_of \<iota>}
+    \<and> concl_of \<iota> < D"
+proof -
+  have "{#} \<notin> N"
+    using bot_ni_n by blast
+  moreover note d_in_n
+  moreover have "\<not> clausal_I_of N |\<approx> D"
+    using n_ent_d by simp
+  moreover have "C \<in> N \<Longrightarrow> \<not> clausal_I_of N |\<approx> C \<Longrightarrow> D \<le> C" for C
+    using d_min[of C] by simp
+  ultimately obtain Cs E where
+    "set Cs \<subseteq> N" and
+    "clausal_I_of N |\<approx>s set Cs" and
+    "Infer (Cs @ [D]) E \<in> Inf" and
+    "\<not> clausal_I_of N |\<approx> E" and
+    "E < D"
+    using clausal_Inf_cex_reducing by metis
+  thus ?thesis
+    using snoc_eq_iff_butlast by fastforce
+qed
+
+sublocale cex_red_inference_system Bot entails Inf I_of
+  by unfold_locales (fact Inf_cex_reducing)
+
+end
+
+end
